tests/snapshots/legacy/dyn/lib/fstar/New_tests.Legacy__dyn__lib.fst
@@ -30,14 +30,14 @@ let print (a: dyn 1 (fun z -> t_Printable z Alloc.String.t_String)) : Prims.unit
     Alloc.String.t_String
   in
   let args:t_Array Core_models.Fmt.Rt.t_Argument (mk_usize 1) =
-    let list = [Core_models.Fmt.Rt.impl__new_display #Alloc.String.t_String args] in
+    let unfold list = [Core_models.Fmt.Rt.impl__new_display #Alloc.String.t_String args] in
     FStar.Pervasives.assert_norm (Prims.eq2 (List.Tot.length list) 1);
     Rust_primitives.Hax.array_of_list 1 list
   in
   let _:Prims.unit =
     Std.Io.Stdio.e_print (Core_models.Fmt.Rt.impl_1__new_v1 (mk_usize 2)
           (mk_usize 1)
-          (let list = [""; "\n"] in
+          (let unfold list = [""; "\n"] in
             FStar.Pervasives.assert_norm (Prims.eq2 (List.Tot.length list) 2);
             Rust_primitives.Hax.array_of_list 2 list)
           args
