tests/snapshots/rustc-coverage/assert/fstar/New_tests.Rustc_coverage__assert.fst
@@ -6,14 +6,14 @@ open Core_models
 let might_fail_assert (one_plus_one: u32) : Prims.unit =
   let args:u32 = one_plus_one <: u32 in
   let args:t_Array Core_models.Fmt.Rt.t_Argument (mk_usize 1) =
-    let list = [Core_models.Fmt.Rt.impl__new_display #u32 args] in
+    let unfold list = [Core_models.Fmt.Rt.impl__new_display #u32 args] in
     FStar.Pervasives.assert_norm (Prims.eq2 (List.Tot.length list) 1);
     Rust_primitives.Hax.array_of_list 1 list
   in
   let _:Prims.unit =
     Std.Io.Stdio.e_print (Core_models.Fmt.Rt.impl_1__new_v1 (mk_usize 2)
           (mk_usize 1)
-          (let list = ["does 1 + 1 = "; "?\n"] in
+          (let unfold list = ["does 1 + 1 = "; "?\n"] in
             FStar.Pervasives.assert_norm (Prims.eq2 (List.Tot.length list) 2);
             Rust_primitives.Hax.array_of_list 2 list)
           args
