tests/snapshots/rustc-coverage/drop_trait/fstar/New_tests.Rustc_coverage__drop_trait.fst
@@ -15,14 +15,14 @@ let impl: Core_models.Ops.Drop.t_Drop t_Firework =
     fun (self: t_Firework) ->
       let args:i32 = self.f_strength <: i32 in
       let args:t_Array Core_models.Fmt.Rt.t_Argument (mk_usize 1) =
-        let list = [Core_models.Fmt.Rt.impl__new_display #i32 args] in
+        let unfold list = [Core_models.Fmt.Rt.impl__new_display #i32 args] in
         FStar.Pervasives.assert_norm (Prims.eq2 (List.Tot.length list) 1);
         Rust_primitives.Hax.array_of_list 1 list
       in
       let _:Prims.unit =
         Std.Io.Stdio.e_print (Core_models.Fmt.Rt.impl_1__new_v1 (mk_usize 2)
               (mk_usize 1)
-              (let list = ["BOOM times "; "!!!\n"] in
+              (let unfold list = ["BOOM times "; "!!!\n"] in
                 FStar.Pervasives.assert_norm (Prims.eq2 (List.Tot.length list) 2);
                 Rust_primitives.Hax.array_of_list 2 list)
               args
@@ -40,7 +40,7 @@ let main (_: Prims.unit) : Core_models.Result.t_Result Prims.unit u8 =
   then
     let _:Prims.unit =
       Std.Io.Stdio.e_print (Core_models.Fmt.Rt.impl_1__new_const (mk_usize 1)
-            (let list = ["Exiting with error...\n"] in
+            (let unfold list = ["Exiting with error...\n"] in
               FStar.Pervasives.assert_norm (Prims.eq2 (List.Tot.length list) 1);
               Rust_primitives.Hax.array_of_list 1 list)
           <:
