tests/snapshots/rustc-coverage/inline/fstar/New_tests.Rustc_coverage__inline.fst
@@ -36,14 +36,14 @@ let display
           let x:v_T = x in
           let args:v_T = x <: v_T in
           let args:t_Array Core_models.Fmt.Rt.t_Argument (mk_usize 1) =
-            let list = [Core_models.Fmt.Rt.impl__new_display #v_T args] in
+            let unfold list = [Core_models.Fmt.Rt.impl__new_display #v_T args] in
             FStar.Pervasives.assert_norm (Prims.eq2 (List.Tot.length list) 1);
             Rust_primitives.Hax.array_of_list 1 list
           in
           let _:Prims.unit =
             Std.Io.Stdio.e_print (Core_models.Fmt.Rt.impl_1__new_v1 (mk_usize 1)
                   (mk_usize 1)
-                  (let list = [""] in
+                  (let unfold list = [""] in
                     FStar.Pervasives.assert_norm (Prims.eq2 (List.Tot.length list) 1);
                     Rust_primitives.Hax.array_of_list 1 list)
                   args
@@ -54,7 +54,7 @@ let display
   in
   let _:Prims.unit =
     Std.Io.Stdio.e_print (Core_models.Fmt.Rt.impl_1__new_const (mk_usize 1)
-          (let list = ["\n"] in
+          (let unfold list = ["\n"] in
             FStar.Pervasives.assert_norm (Prims.eq2 (List.Tot.length list) 1);
             Rust_primitives.Hax.array_of_list 1 list)
         <:
@@ -66,7 +66,7 @@ let display
 let error (_: Prims.unit) : Prims.unit =
   Rust_primitives.Hax.never_to_any (Core_models.Panicking.panic_fmt (Core_models.Fmt.Rt.impl_1__new_const
             (mk_usize 1)
-            (let list = ["error"] in
+            (let unfold list = ["error"] in
               FStar.Pervasives.assert_norm (Prims.eq2 (List.Tot.length list) 1);
               Rust_primitives.Hax.array_of_list 1 list)
           <:
@@ -133,7 +133,7 @@ let permutations
 let main (_: Prims.unit) : Prims.unit =
   let _:Prims.unit =
     permutations #FStar.Char.char
-      ((let list = ['a'; 'b'; 'c'] in
+      ((let unfold list = ['a'; 'b'; 'c'] in
           FStar.Pervasives.assert_norm (Prims.eq2 (List.Tot.length list) 3);
           Rust_primitives.Hax.array_of_list 3 list)
         <:
