tests/snapshots/rustc-coverage/inner_items/fstar/New_tests.Rustc_coverage__inner_items.fst
@@ -16,14 +16,14 @@ let main__in_func (a: u32) : Prims.unit =
   let c:u32 = a +! b in
   let args:u32 = c <: u32 in
   let args:t_Array Core_models.Fmt.Rt.t_Argument (mk_usize 1) =
-    let list = [Core_models.Fmt.Rt.impl__new_display #u32 args] in
+    let unfold list = [Core_models.Fmt.Rt.impl__new_display #u32 args] in
     FStar.Pervasives.assert_norm (Prims.eq2 (List.Tot.length list) 1);
     Rust_primitives.Hax.array_of_list 1 list
   in
   let _:Prims.unit =
     Std.Io.Stdio.e_print (Core_models.Fmt.Rt.impl_1__new_v1 (mk_usize 2)
           (mk_usize 1)
-          (let list = ["c = "; "\n"] in
+          (let unfold list = ["c = "; "\n"] in
             FStar.Pervasives.assert_norm (Prims.eq2 (List.Tot.length list) 2);
             Rust_primitives.Hax.array_of_list 2 list)
           args
