tests/snapshots/rustc-coverage/issue-84561/fstar/New_tests.Rustc_coverage__issue_84561_.fst
@@ -53,7 +53,7 @@ let impl: Core_models.Fmt.t_Debug t_Foo =
       (out: Core_models.Result.t_Result Prims.unit Core_models.Fmt.t_Error) =
         Core_models.Fmt.impl_11__write_fmt f
           (Core_models.Fmt.Rt.impl_1__new_const (mk_usize 1)
-              (let list = ["try and succeed"] in
+              (let unfold list = ["try and succeed"] in
                 FStar.Pervasives.assert_norm (Prims.eq2 (List.Tot.length list) 1);
                 Rust_primitives.Hax.array_of_list 1 list)
             <:
@@ -103,14 +103,14 @@ let test3 (_: Prims.unit) : Prims.unit =
   in
   let args:t_Foo = (Foo (mk_u32 1) <: t_Foo) <: t_Foo in
   let args:t_Array Core_models.Fmt.Rt.t_Argument (mk_usize 1) =
-    let list = [Core_models.Fmt.Rt.impl__new_debug #t_Foo args] in
+    let unfold list = [Core_models.Fmt.Rt.impl__new_debug #t_Foo args] in
     FStar.Pervasives.assert_norm (Prims.eq2 (List.Tot.length list) 1);
     Rust_primitives.Hax.array_of_list 1 list
   in
   let _:Prims.unit =
     Std.Io.Stdio.e_print (Core_models.Fmt.Rt.impl_1__new_v1 (mk_usize 2)
           (mk_usize 1)
-          (let list = [""; "\n"] in
+          (let unfold list = [""; "\n"] in
             FStar.Pervasives.assert_norm (Prims.eq2 (List.Tot.length list) 2);
             Rust_primitives.Hax.array_of_list 2 list)
           args
@@ -120,14 +120,14 @@ let test3 (_: Prims.unit) : Prims.unit =
   let _:Prims.unit = () in
   let args:t_Foo = bar <: t_Foo in
   let args:t_Array Core_models.Fmt.Rt.t_Argument (mk_usize 1) =
-    let list = [Core_models.Fmt.Rt.impl__new_debug #t_Foo args] in
+    let unfold list = [Core_models.Fmt.Rt.impl__new_debug #t_Foo args] in
     FStar.Pervasives.assert_norm (Prims.eq2 (List.Tot.length list) 1);
     Rust_primitives.Hax.array_of_list 1 list
   in
   let _:Prims.unit =
     Std.Io.Stdio.e_print (Core_models.Fmt.Rt.impl_1__new_v1 (mk_usize 2)
           (mk_usize 1)
-          (let list = [""; "\n"] in
+          (let unfold list = [""; "\n"] in
             FStar.Pervasives.assert_norm (Prims.eq2 (List.Tot.length list) 2);
             Rust_primitives.Hax.array_of_list 2 list)
           args
@@ -137,14 +137,14 @@ let test3 (_: Prims.unit) : Prims.unit =
   let _:Prims.unit = () in
   let args:t_Foo = baz <: t_Foo in
   let args:t_Array Core_models.Fmt.Rt.t_Argument (mk_usize 1) =
-    let list = [Core_models.Fmt.Rt.impl__new_debug #t_Foo args] in
+    let unfold list = [Core_models.Fmt.Rt.impl__new_debug #t_Foo args] in
     FStar.Pervasives.assert_norm (Prims.eq2 (List.Tot.length list) 1);
     Rust_primitives.Hax.array_of_list 1 list
   in
   let _:Prims.unit =
     Std.Io.Stdio.e_print (Core_models.Fmt.Rt.impl_1__new_v1 (mk_usize 2)
           (mk_usize 1)
-          (let list = [""; "\n"] in
+          (let unfold list = [""; "\n"] in
             FStar.Pervasives.assert_norm (Prims.eq2 (List.Tot.length list) 2);
             Rust_primitives.Hax.array_of_list 2 list)
           args
@@ -179,14 +179,14 @@ let test3 (_: Prims.unit) : Prims.unit =
   in
   let args:t_Foo = bar <: t_Foo in
   let args:t_Array Core_models.Fmt.Rt.t_Argument (mk_usize 1) =
-    let list = [Core_models.Fmt.Rt.impl__new_debug #t_Foo args] in
+    let unfold list = [Core_models.Fmt.Rt.impl__new_debug #t_Foo args] in
     FStar.Pervasives.assert_norm (Prims.eq2 (List.Tot.length list) 1);
     Rust_primitives.Hax.array_of_list 1 list
   in
   let _:Prims.unit =
     Std.Io.Stdio.e_print (Core_models.Fmt.Rt.impl_1__new_v1 (mk_usize 2)
           (mk_usize 1)
-          (let list = [""; "\n"] in
+          (let unfold list = [""; "\n"] in
             FStar.Pervasives.assert_norm (Prims.eq2 (List.Tot.length list) 2);
             Rust_primitives.Hax.array_of_list 2 list)
           args
@@ -196,14 +196,14 @@ let test3 (_: Prims.unit) : Prims.unit =
   let _:Prims.unit = () in
   let args:t_Foo = (Foo (mk_u32 1) <: t_Foo) <: t_Foo in
   let args:t_Array Core_models.Fmt.Rt.t_Argument (mk_usize 1) =
-    let list = [Core_models.Fmt.Rt.impl__new_debug #t_Foo args] in
+    let unfold list = [Core_models.Fmt.Rt.impl__new_debug #t_Foo args] in
     FStar.Pervasives.assert_norm (Prims.eq2 (List.Tot.length list) 1);
     Rust_primitives.Hax.array_of_list 1 list
   in
   let _:Prims.unit =
     Std.Io.Stdio.e_print (Core_models.Fmt.Rt.impl_1__new_v1 (mk_usize 2)
           (mk_usize 1)
-          (let list = [""; "\n"] in
+          (let unfold list = [""; "\n"] in
             FStar.Pervasives.assert_norm (Prims.eq2 (List.Tot.length list) 2);
             Rust_primitives.Hax.array_of_list 2 list)
           args
@@ -389,7 +389,7 @@ let test1 (_: Prims.unit) : Prims.unit =
     then
       let _:Prims.unit =
         Std.Io.Stdio.e_print (Core_models.Fmt.Rt.impl_1__new_const (mk_usize 1)
-              (let list = ["debug is enabled\n"] in
+              (let unfold list = ["debug is enabled\n"] in
                 FStar.Pervasives.assert_norm (Prims.eq2 (List.Tot.length list) 1);
                 Rust_primitives.Hax.array_of_list 1 list)
             <:
@@ -406,7 +406,7 @@ let test1 (_: Prims.unit) : Prims.unit =
     then
       let _:Prims.unit =
         Std.Io.Stdio.e_print (Core_models.Fmt.Rt.impl_1__new_const (mk_usize 1)
-              (let list = ["debug is enabled\n"] in
+              (let unfold list = ["debug is enabled\n"] in
                 FStar.Pervasives.assert_norm (Prims.eq2 (List.Tot.length list) 1);
                 Rust_primitives.Hax.array_of_list 1 list)
             <:
@@ -424,7 +424,7 @@ let test1 (_: Prims.unit) : Prims.unit =
     then
       let _:Prims.unit =
         Std.Io.Stdio.e_print (Core_models.Fmt.Rt.impl_1__new_const (mk_usize 1)
-              (let list = ["debug is enabled\n"] in
+              (let unfold list = ["debug is enabled\n"] in
                 FStar.Pervasives.assert_norm (Prims.eq2 (List.Tot.length list) 1);
                 Rust_primitives.Hax.array_of_list 1 list)
             <:
@@ -447,7 +447,7 @@ let test1 (_: Prims.unit) : Prims.unit =
     then
       let _:Prims.unit =
         Std.Io.Stdio.e_print (Core_models.Fmt.Rt.impl_1__new_const (mk_usize 1)
-              (let list = ["debug is enabled\n"] in
+              (let unfold list = ["debug is enabled\n"] in
                 FStar.Pervasives.assert_norm (Prims.eq2 (List.Tot.length list) 1);
                 Rust_primitives.Hax.array_of_list 1 list)
             <:
@@ -462,14 +462,14 @@ let test1 (_: Prims.unit) : Prims.unit =
 let test2__call_print (s: string) : Prims.unit =
   let args:string = s <: string in
   let args:t_Array Core_models.Fmt.Rt.t_Argument (mk_usize 1) =
-    let list = [Core_models.Fmt.Rt.impl__new_display #string args] in
+    let unfold list = [Core_models.Fmt.Rt.impl__new_display #string args] in
     FStar.Pervasives.assert_norm (Prims.eq2 (List.Tot.length list) 1);
     Rust_primitives.Hax.array_of_list 1 list
   in
   let _:Prims.unit =
     Std.Io.Stdio.e_print (Core_models.Fmt.Rt.impl_1__new_v1 (mk_usize 1)
           (mk_usize 1)
-          (let list = [""] in
+          (let unfold list = [""] in
             FStar.Pervasives.assert_norm (Prims.eq2 (List.Tot.length list) 1);
             Rust_primitives.Hax.array_of_list 1 list)
           args
@@ -490,7 +490,7 @@ let test2 (_: Prims.unit) : Prims.unit =
     then
       let _:Prims.unit =
         Std.Io.Stdio.e_print (Core_models.Fmt.Rt.impl_1__new_const (mk_usize 1)
-              (let list = ["debug is enabled\n"] in
+              (let unfold list = ["debug is enabled\n"] in
                 FStar.Pervasives.assert_norm (Prims.eq2 (List.Tot.length list) 1);
                 Rust_primitives.Hax.array_of_list 1 list)
             <:
