tests/snapshots/rustc-coverage/loops_branches/fstar/New_tests.Rustc_coverage__loops_branches.fst
@@ -46,7 +46,7 @@ let impl: Core_models.Fmt.t_Debug t_DebugTest =
         (out: Core_models.Result.t_Result Prims.unit Core_models.Fmt.t_Error) =
           Core_models.Fmt.impl_11__write_fmt f
             (Core_models.Fmt.Rt.impl_1__new_const (mk_usize 1)
-                (let list = ["cool"] in
+                (let unfold list = ["cool"] in
                   FStar.Pervasives.assert_norm (Prims.eq2 (List.Tot.length list) 1);
                   Rust_primitives.Hax.array_of_list 1 list)
               <:
@@ -91,7 +91,7 @@ let impl: Core_models.Fmt.t_Debug t_DebugTest =
                       (out: Core_models.Result.t_Result Prims.unit Core_models.Fmt.t_Error) =
                         Core_models.Fmt.impl_11__write_fmt f
                           (Core_models.Fmt.Rt.impl_1__new_const (mk_usize 1)
-                              (let list = ["cool"] in
+                              (let unfold list = ["cool"] in
                                 FStar.Pervasives.assert_norm (Prims.eq2 (List.Tot.length list) 1);
                                 Rust_primitives.Hax.array_of_list 1 list)
                             <:
@@ -201,7 +201,7 @@ let impl: Core_models.Fmt.t_Debug t_DebugTest =
                   (out: Core_models.Result.t_Result Prims.unit Core_models.Fmt.t_Error) =
                     Core_models.Fmt.impl_11__write_fmt f
                       (Core_models.Fmt.Rt.impl_1__new_const (mk_usize 1)
-                          (let list = ["cool"] in
+                          (let unfold list = ["cool"] in
                             FStar.Pervasives.assert_norm (Prims.eq2 (List.Tot.length list) 1);
                             Rust_primitives.Hax.array_of_list 1 list)
                         <:
@@ -330,7 +330,7 @@ let impl_1: Core_models.Fmt.t_Display t_DisplayTest =
                   (out: Core_models.Result.t_Result Prims.unit Core_models.Fmt.t_Error) =
                     Core_models.Fmt.impl_11__write_fmt f
                       (Core_models.Fmt.Rt.impl_1__new_const (mk_usize 1)
-                          (let list = ["cool"] in
+                          (let unfold list = ["cool"] in
                             FStar.Pervasives.assert_norm (Prims.eq2 (List.Tot.length list) 1);
                             Rust_primitives.Hax.array_of_list 1 list)
                         <:
@@ -407,7 +407,7 @@ let impl_1: Core_models.Fmt.t_Display t_DisplayTest =
         (out: Core_models.Result.t_Result Prims.unit Core_models.Fmt.t_Error) =
           Core_models.Fmt.impl_11__write_fmt f
             (Core_models.Fmt.Rt.impl_1__new_const (mk_usize 1)
-                (let list = ["cool"] in
+                (let unfold list = ["cool"] in
                   FStar.Pervasives.assert_norm (Prims.eq2 (List.Tot.length list) 1);
                   Rust_primitives.Hax.array_of_list 1 list)
               <:
@@ -460,7 +460,7 @@ let impl_1: Core_models.Fmt.t_Display t_DisplayTest =
                       (out: Core_models.Result.t_Result Prims.unit Core_models.Fmt.t_Error) =
                         Core_models.Fmt.impl_11__write_fmt f
                           (Core_models.Fmt.Rt.impl_1__new_const (mk_usize 1)
-                              (let list = ["cool"] in
+                              (let unfold list = ["cool"] in
                                 FStar.Pervasives.assert_norm (Prims.eq2 (List.Tot.length list) 1);
                                 Rust_primitives.Hax.array_of_list 1 list)
                             <:
@@ -533,14 +533,14 @@ let main (_: Prims.unit) : Prims.unit =
   let debug_test:t_DebugTest = DebugTest <: t_DebugTest in
   let args:t_DebugTest = debug_test <: t_DebugTest in
   let args:t_Array Core_models.Fmt.Rt.t_Argument (mk_usize 1) =
-    let list = [Core_models.Fmt.Rt.impl__new_debug #t_DebugTest args] in
+    let unfold list = [Core_models.Fmt.Rt.impl__new_debug #t_DebugTest args] in
     FStar.Pervasives.assert_norm (Prims.eq2 (List.Tot.length list) 1);
     Rust_primitives.Hax.array_of_list 1 list
   in
   let _:Prims.unit =
     Std.Io.Stdio.e_print (Core_models.Fmt.Rt.impl_1__new_v1 (mk_usize 2)
           (mk_usize 1)
-          (let list = [""; "\n"] in
+          (let unfold list = [""; "\n"] in
             FStar.Pervasives.assert_norm (Prims.eq2 (List.Tot.length list) 2);
             Rust_primitives.Hax.array_of_list 2 list)
           args
@@ -551,14 +551,14 @@ let main (_: Prims.unit) : Prims.unit =
   let display_test:t_DisplayTest = DisplayTest <: t_DisplayTest in
   let args:t_DisplayTest = display_test <: t_DisplayTest in
   let args:t_Array Core_models.Fmt.Rt.t_Argument (mk_usize 1) =
-    let list = [Core_models.Fmt.Rt.impl__new_display #t_DisplayTest args] in
+    let unfold list = [Core_models.Fmt.Rt.impl__new_display #t_DisplayTest args] in
     FStar.Pervasives.assert_norm (Prims.eq2 (List.Tot.length list) 1);
     Rust_primitives.Hax.array_of_list 1 list
   in
   let _:Prims.unit =
     Std.Io.Stdio.e_print (Core_models.Fmt.Rt.impl_1__new_v1 (mk_usize 2)
           (mk_usize 1)
-          (let list = [""; "\n"] in
+          (let unfold list = [""; "\n"] in
             FStar.Pervasives.assert_norm (Prims.eq2 (List.Tot.length list) 2);
             Rust_primitives.Hax.array_of_list 2 list)
           args
