tests/snapshots/rustc-coverage/attr/trait-impl-inherit/fstar/New_tests.Rustc_coverage__attr__trait_impl_inherit.fst
@@ -64,7 +64,7 @@ let impl: t_T t_S =
     fun (self: t_S) ->
       let _:Prims.unit =
         Std.Io.Stdio.e_print (Core_models.Fmt.Rt.impl_1__new_const (mk_usize 1)
-              (let list = ["impl S\n"] in
+              (let unfold list = ["impl S\n"] in
                 FStar.Pervasives.assert_norm (Prims.eq2 (List.Tot.length list) 1);
                 Rust_primitives.Hax.array_of_list 1 list)
             <:
