tests/snapshots/rustc-coverage/branch/generics/fstar/New_tests.Rustc_coverage__branch__generics.fst
@@ -7,7 +7,7 @@ let print_size (#v_T: Type0) (_: Prims.unit) : Prims.unit =
   then
     let _:Prims.unit =
       Std.Io.Stdio.e_print (Core_models.Fmt.Rt.impl_1__new_const (mk_usize 1)
-            (let list = ["size > 4\n"] in
+            (let unfold list = ["size > 4\n"] in
               FStar.Pervasives.assert_norm (Prims.eq2 (List.Tot.length list) 1);
               Rust_primitives.Hax.array_of_list 1 list)
           <:
@@ -18,7 +18,7 @@ let print_size (#v_T: Type0) (_: Prims.unit) : Prims.unit =
   else
     let _:Prims.unit =
       Std.Io.Stdio.e_print (Core_models.Fmt.Rt.impl_1__new_const (mk_usize 1)
-            (let list = ["size <= 4\n"] in
+            (let unfold list = ["size <= 4\n"] in
               FStar.Pervasives.assert_norm (Prims.eq2 (List.Tot.length list) 1);
               Rust_primitives.Hax.array_of_list 1 list)
           <:
