tests/snapshots/rustc-coverage/branch/lazy-boolean/fstar/New_tests.Rustc_coverage__branch__lazy_boolean.fst
@@ -88,7 +88,7 @@ let main (_: Prims.unit) : (Prims.unit & Prims.unit) =
     Core_models.Iter.Traits.Iterator.f_fold (Core_models.Iter.Traits.Collect.f_into_iter #(t_Array
               bool (mk_usize 5))
           #FStar.Tactics.Typeclasses.solve
-          (let list = [false; true; true; true; true] in
+          (let unfold list = [false; true; true; true; true] in
             FStar.Pervasives.assert_norm (Prims.eq2 (List.Tot.length list) 5);
             Rust_primitives.Hax.array_of_list 5 list)
         <:
@@ -100,7 +100,7 @@ let main (_: Prims.unit) : (Prims.unit & Prims.unit) =
           Core_models.Iter.Traits.Iterator.f_fold (Core_models.Iter.Traits.Collect.f_into_iter #(t_Array
                     bool (mk_usize 3))
                 #FStar.Tactics.Typeclasses.solve
-                (let list = [false; true; true] in
+                (let unfold list = [false; true; true] in
                   FStar.Pervasives.assert_norm (Prims.eq2 (List.Tot.length list) 3);
                   Rust_primitives.Hax.array_of_list 3 list)
               <:
