tests/snapshots/rustc-coverage/unicode/fstar/New_tests.Rustc_coverage__unicode.fst
@@ -29,7 +29,7 @@ let main (_: Prims.unit) : Prims.unit =
     then
       let _:Prims.unit =
         Std.Io.Stdio.e_print (Core_models.Fmt.Rt.impl_1__new_const (mk_usize 1)
-              (let list = ["true\n"] in
+              (let unfold list = ["true\n"] in
                 FStar.Pervasives.assert_norm (Prims.eq2 (List.Tot.length list) 1);
                 Rust_primitives.Hax.array_of_list 1 list)
             <:
