tests/snapshots/rustc-coverage/unused_mod/fstar/New_tests.Rustc_coverage__unused_mod.fst
@@ -5,7 +5,7 @@ open Core_models
 let main (_: Prims.unit) : Prims.unit =
   let _:Prims.unit =
     Std.Io.Stdio.e_print (Core_models.Fmt.Rt.impl_1__new_const (mk_usize 1)
-          (let list = ["hello world!\n"] in
+          (let unfold list = ["hello world!\n"] in
             FStar.Pervasives.assert_norm (Prims.eq2 (List.Tot.length list) 1);
             Rust_primitives.Hax.array_of_list 1 list)
         <:
